tests/lean/1327.lean
@@ -1,4 +1,4 @@
 example (n) : nat.pred n = n :=
 begin
-  dsimp
+  dsimp {fail_if_unchaged := ff}
 end
